Continue

src/Realisation.thy
@@ -1,4 +1,4 @@
-theory Realization
+theory Realisation
   imports ZFC_Extras Graph_Theory.Graph_Theory
 begin
 
@@ -62,7 +62,7 @@ lemma card_ancestors_strict_mono:
 
 end
 
-locale realization = dag G for G +
+locale realisation = dag G for G +
   fixes P T :: "'a set"
   fixes I :: "'a \<Rightarrow> V"
   assumes P_T_partition_verts: "P \<inter> T = {}" "verts G = P \<union> T"
@@ -93,15 +93,15 @@ proof(cases t rule: height.cases)
     by auto
 qed simp_all
 
-function realize :: "'a \<Rightarrow> V" where
-  "x \<in> P \<Longrightarrow> realize x = vset {I x}"
-| "t \<in> T \<Longrightarrow> realize t = vset (realize ` parents G t)"
-| "x \<notin> P \<union> T \<Longrightarrow> realize x = 0"
+function realise :: "'a \<Rightarrow> V" where
+  "x \<in> P \<Longrightarrow> realise x = vset {I x}"
+| "t \<in> T \<Longrightarrow> realise t = vset (realise ` parents G t)"
+| "x \<notin> P \<union> T \<Longrightarrow> realise x = 0"
   using P_T_partition_verts by auto
 termination
   by (relation "measure (\<lambda>t. card (ancestors G t))") (simp_all add: card_ancestors_strict_mono)
 
-lemma small_realization_parents[simp, intro!]: "small (realize ` parents G t)"
+lemma small_realisation_parents[simp, intro!]: "small (realise ` parents G t)"
   using small_parents by auto
 
 lemma lemma1_1:
@@ -116,22 +116,22 @@ proof(cases t rule: height.cases)
 qed (use P_T_partition_verts in auto)
 
 
-lemma dominates_if_mem_realization:
-  assumes "\<forall>x \<in> P. \<forall>y \<in> P \<union> T. x \<noteq> y \<longrightarrow> I x \<noteq> realize y"
+lemma dominates_if_mem_realisation:
+  assumes "\<forall>x \<in> P. \<forall>y \<in> P \<union> T. x \<noteq> y \<longrightarrow> I x \<noteq> realise y"
   assumes "s \<in> P \<union> T" "t \<in> P \<union> T"
-  assumes "realize s \<in> elts (realize t)"
-  obtains s' where "s' \<rightarrow>\<^bsub>G\<^esub> t" "realize s = realize s'"
+  assumes "realise s \<in> elts (realise t)"
+  obtains s' where "s' \<rightarrow>\<^bsub>G\<^esub> t" "realise s = realise s'"
   using assms(2-)
-proof(induction t rule: realize.induct)
+proof(induction t rule: realise.induct)
   case (1 x)
   with assms(1) show ?case 
-    by (metis all_not_in_conv elts_of_set insert_iff mem_not_sym realize.simps(1))
+    by (metis all_not_in_conv elts_of_set insert_iff mem_not_sym realise.simps(1))
 qed auto
 
 lemma lemma1_2':
   assumes "inj_on I P"
-  assumes "\<forall>x \<in> P. \<forall>y \<in> P \<union> T. x \<noteq> y \<longrightarrow> I x \<noteq> realize y"
-  assumes "t1 \<in> P \<union> T" "t2 \<in> P \<union> T" "realize t1 = realize t2"
+  assumes "\<forall>x \<in> P. \<forall>y \<in> P \<union> T. x \<noteq> y \<longrightarrow> I x \<noteq> realise y"
+  assumes "t1 \<in> P \<union> T" "t2 \<in> P \<union> T" "realise t1 = realise t2"
   shows "height t1 \<le> height t2"
 proof -
   from assms(3,4) consider "t1 \<in> P" | "t1 \<in> T" "t2 \<in> P" | "t1 \<in> T" "t2 \<in> T"
@@ -145,13 +145,13 @@ proof -
     then show ?thesis
     proof(cases t1 rule: height.cases)
       case (3 t s)
-      have "small (realize ` parents G t1)"
+      have "small (realise ` parents G t1)"
         by blast+
-      with 2 3 assms(5) have "realize ` parents G t1 = {I t2}"
-        using \<open>small (realize ` parents G t1)\<close> by force
+      with 2 3 assms(5) have "realise ` parents G t1 = {I t2}"
+        using \<open>small (realise ` parents G t1)\<close> by force
       moreover from 3 adj_in_verts P_T_partition_verts have "s \<in> P \<union> T"
         by simp
-      then have "I t2 \<noteq> realize s"
+      then have "I t2 \<noteq> realise s"
         using 2 3 assms(2,3,5) by metis
       ultimately show ?thesis
         using 3 by (metis ex_in_conv imageI insert_iff mem_Collect_eq)
@@ -170,7 +170,7 @@ proof -
         with less.prems assms(2) show ?thesis
           using P_T_partition_verts(1)
           apply(cases t2 rule: height_cases'; cases t1 rule: height_cases')
-          by (auto simp: vset_eq_0_iff[OF small_realization_parents])
+          by (auto simp: vset_eq_0_iff[OF small_realisation_parents])
       next
         case (Suc x)
         then have "t2 \<notin> P"
@@ -180,10 +180,10 @@ proof -
           case (nP_Suc s)
           with P_T_partition_verts adj_in_verts(1) have "s \<in> P \<union> T"
             by blast
-          from nP_Suc less.prems(1) have "realize s \<in> elts (realize t1)"
+          from nP_Suc less.prems(1) have "realise s \<in> elts (realise t1)"
             by auto
-          then obtain s' where s': "realize s' = realize s" "s' \<rightarrow>\<^bsub>G\<^esub> t2"
-            using dominates_if_mem_realization \<open>s \<in> P \<union> T\<close> less.prems assms(2)
+          then obtain s' where s': "realise s' = realise s" "s' \<rightarrow>\<^bsub>G\<^esub> t2"
+            using dominates_if_mem_realisation \<open>s \<in> P \<union> T\<close> less.prems assms(2)
             by (metis Un_iff)
           then have "s' \<in> P \<union> T"
             using P_T_partition_verts(2) adj_in_verts(1) by blast
@@ -203,16 +203,16 @@ proof -
               case (3 _ u)
               then have "u \<in> P \<union> T"
                 using P_T_partition_verts(2) adj_in_verts(1) by blast
-              with 3 that have "realize u \<in> elts (realize s)"
+              with 3 that have "realise u \<in> elts (realise s)"
                 by auto
-              then obtain u' where "u' \<rightarrow>\<^bsub>G\<^esub> s'" "realize u' = realize u"
-                using dominates_if_mem_realization
+              then obtain u' where "u' \<rightarrow>\<^bsub>G\<^esub> s'" "realise u' = realise u"
+                using dominates_if_mem_realisation
                 by (metis \<open>s' \<in> P \<union> T\<close> \<open>u \<in> P \<union> T\<close> assms(2) s'(1))
 
               then show ?thesis
-                using \<open>realize u \<in> elts (realize s)\<close> \<open>s' \<in> P\<close> assms(2) s'(1)
+                using \<open>realise u \<in> elts (realise s)\<close> \<open>s' \<in> P\<close> assms(2) s'(1)
                 by (metis P_T_partition_verts(2)
-                    adj_in_verts(1) elts_of_set mem_not_refl realize.simps(1)
+                    adj_in_verts(1) elts_of_set mem_not_refl realise.simps(1)
                     singletonD small_empty small_insert)
             qed auto
           qed
@@ -228,23 +228,23 @@ qed
 
 lemma lemma1_2:
   assumes "inj_on I P"
-  assumes "\<forall>x \<in> P. \<forall>y \<in> P \<union> T. x \<noteq> y \<longrightarrow> I x \<noteq> realize y"
-  assumes "t1 \<in> P \<union> T" "t2 \<in> P \<union> T" "realize t1 = realize t2"
+  assumes "\<forall>x \<in> P. \<forall>y \<in> P \<union> T. x \<noteq> y \<longrightarrow> I x \<noteq> realise y"
+  assumes "t1 \<in> P \<union> T" "t2 \<in> P \<union> T" "realise t1 = realise t2"
   shows "height t1 = height t2"
   using assms lemma1_2' le_antisym unfolding inj_on_def by metis
 
 lemma lemma1_3:
   assumes "inj_on I P"
-  assumes "\<forall>x \<in> P. \<forall>y \<in> P \<union> T. x \<noteq> y \<longrightarrow> I x \<noteq> realize y"
-  assumes "s \<in> P \<union> T" "t \<in> P \<union> T" "realize s \<in> elts (realize t)"
+  assumes "\<forall>x \<in> P. \<forall>y \<in> P \<union> T. x \<noteq> y \<longrightarrow> I x \<noteq> realise y"
+  assumes "s \<in> P \<union> T" "t \<in> P \<union> T" "realise s \<in> elts (realise t)"
   shows "height s < height t"
 proof -
-  from assms dominates_if_mem_realization obtain s' where
-    s': "realize s' = realize s" "s' \<rightarrow>\<^bsub>G\<^esub> t" by metis
+  from assms dominates_if_mem_realisation obtain s' where
+    s': "realise s' = realise s" "s' \<rightarrow>\<^bsub>G\<^esub> t" by metis
   then have "s' \<in> P \<union> T"
     using adj_in_verts P_T_partition_verts by blast
   from assms(2-5) have "t \<in> T"
-    by (metis elts_of_set mem_not_sym realize.cases realize.simps(1) singletonD
+    by (metis elts_of_set mem_not_sym realise.cases realise.simps(1) singletonD
               small_empty small_insert)
   with lemma1_1[OF \<open>s' \<in> P \<union> T\<close>] assms s' have "height s' < height t"
     by auto
@@ -254,9 +254,9 @@ proof -
     by linarith
 qed
 
-lemma card_realization_T_less_card_verts:
-  "t \<in> T \<Longrightarrow> card (elts (realize t)) < card (P \<union> T)"
-proof(induction t rule: realize.induct)
+lemma card_realisation_T_less_card_verts:
+  "t \<in> T \<Longrightarrow> card (elts (realise t)) < card (P \<union> T)"
+proof(induction t rule: realise.induct)
   case (2 t)
   then have "t \<in> verts G"
     using P_T_partition_verts by simp
@@ -264,21 +264,21 @@ proof(induction t rule: realize.induct)
     using adj_not_same by auto
   from psubset_card_mono[OF _ this] have "card (parents G t) < card (verts G)"
     by simp
-  then have "card (realize ` parents G t) < card (verts G)"
-    using card_image_le[OF finite_parents, where ?f=realize and ?s1=t] by linarith 
+  then have "card (realise ` parents G t) < card (verts G)"
+    using card_image_le[OF finite_parents, where ?f=realise and ?s1=t] by linarith 
   with 2 show ?case
     using P_T_partition_verts(2) by auto
 qed (use P_T_partition_verts in auto)
 
-lemma card_realization_P:
-  "p \<in> P \<Longrightarrow> card (elts (realize p)) = 1"
+lemma card_realisation_P:
+  "p \<in> P \<Longrightarrow> card (elts (realise p)) = 1"
   by simp
 
-lemma card_elts_realization_T:
-  assumes "t \<in> T" "x \<in> elts (realize t)"
+lemma card_elts_realisation_T:
+  assumes "t \<in> T" "x \<in> elts (realise t)"
   shows "card (elts x) < card (P \<union> T)"
 proof -
-  obtain s where s: "x = realize s" "s \<in> parents G t"
+  obtain s where s: "x = realise s" "s \<in> parents G t"
     using assms by force
   then have "s \<in> P \<union> T"
     using P_T_partition_verts(2) adj_in_verts(1) by blast
@@ -287,7 +287,7 @@ proof -
   with finite_P_un_T have "card (P \<union> T) \<ge> 2"
     by (metis card_2_iff card_mono)
   with \<open>s \<in> P \<union> T\<close> s show ?thesis
-    using card_realization_T_less_card_verts
+    using card_realisation_T_less_card_verts
     by auto
 qed
 
